thys/ConcurrentIMP/CIMP_pred.thy
@@ -15,122 +15,123 @@ imports
 begin
 
 (*>*)
-section\<open>Lifted predicates\<close>
+section\<open> Point-free notation \<close>
 
 text\<open>
 
 \label{sec:cimp-lifted-predicates}
 
 Typically we define predicates as functions of a state. The following
-provide a somewhat comfortable imitatation of Isabelle/HOL's
+provide a somewhat comfortable point-free imitation of Isabelle/HOL's
 operators.
 
 \<close>
-
-(*
-FIXME precedences probably need tweaking. @{text "pred_diff"}
-FIXME consider bounded quantifiers. See Set.thy. Don't care about printing so maybe not too hard.
-*)
-
-abbreviation (input)
-  pred_pair :: "('a \<Rightarrow> 'b) \<Rightarrow> ('a \<Rightarrow> 'c) \<Rightarrow> 'a \<Rightarrow> 'b \<times> 'c" (infixr "\<otimes>" 60) where
-  "a \<otimes> b \<equiv> \<lambda>s. (a s, b s)"
-
-abbreviation (input)
-  pred_in :: "('a \<Rightarrow> 'b) \<Rightarrow> ('a \<Rightarrow> 'b set) \<Rightarrow> 'a \<Rightarrow> bool" (infix "in" 50) where
-  "a in A \<equiv> \<lambda>s. a s \<in> A s"
-
-abbreviation (input)
-  pred_subseteq :: "('a \<Rightarrow> 'b set) \<Rightarrow> ('a \<Rightarrow> 'b set) \<Rightarrow> 'a \<Rightarrow> bool" (infix "subseteq" 50) where
-  "A subseteq B \<equiv> \<lambda>s. A s \<subseteq> B s"
-
-abbreviation (input)
-  pred_union :: "('a \<Rightarrow> 'b set) \<Rightarrow> ('a \<Rightarrow> 'b set) \<Rightarrow> 'a \<Rightarrow> 'b set" (infixl "union" 65) where
-  "a union b \<equiv> \<lambda>s. a s \<union> b s"
-
-abbreviation (input)
-  pred_diff :: "('a \<Rightarrow> 'b set) \<Rightarrow> ('a \<Rightarrow> 'b set) \<Rightarrow> 'a \<Rightarrow> 'b set" (infixr "diff" 65) where
-  "a diff b \<equiv> \<lambda>s. a s - b s"
-
-abbreviation (input)
-  pred_comp :: "(('b \<Rightarrow> 'c) \<Rightarrow> 'a \<Rightarrow> 'd) \<Rightarrow> ('b \<Rightarrow> 'a \<Rightarrow> 'c) \<Rightarrow> 'a \<Rightarrow> 'd" (infixl "\<bigcirc>" 55) where
-  "f \<bigcirc> g \<equiv> \<lambda>s. f (\<lambda>b. g b s) s"
-
-abbreviation (input)
-  pred_app :: "('b \<Rightarrow> 'a \<Rightarrow> 'c) \<Rightarrow> ('a \<Rightarrow> 'b) \<Rightarrow> 'a \<Rightarrow> 'c" (infixl "\<triangleright>" 100) where
-  "f \<triangleright> g \<equiv> \<lambda>s. f (g s) s"
-
-abbreviation (input)
-  pred_eq :: "('a \<Rightarrow> 'b) \<Rightarrow> ('a \<Rightarrow> 'b) \<Rightarrow> 'a \<Rightarrow> bool" (infix "eq" 40) where
-  "a eq b \<equiv> \<lambda>s. a s = b s"
-
-abbreviation (input)
-  pred_neq :: "('a \<Rightarrow> 'b) \<Rightarrow> ('a \<Rightarrow> 'b) \<Rightarrow> 'a \<Rightarrow> bool" (infix "neq" 40) where
-  "a neq b \<equiv> \<lambda>s. a s \<noteq> b s"
-
-abbreviation (input)
-  pred_lt :: "('a \<Rightarrow> 'b::ord) \<Rightarrow> ('a \<Rightarrow> 'b) \<Rightarrow> 'a \<Rightarrow> bool" (infix "lt" 40) where
-  "a lt b \<equiv> \<lambda>s. a s < b s"
-
-abbreviation (input)
-  pred_and :: "('a \<Rightarrow> bool) \<Rightarrow> ('a \<Rightarrow> bool) \<Rightarrow> 'a \<Rightarrow> bool" (infixr "and" 35) where
-  "a and b \<equiv> \<lambda>s. a s \<and> b s"
-
-abbreviation (input)
-  pred_or :: "('a \<Rightarrow> bool) \<Rightarrow> ('a \<Rightarrow> bool) \<Rightarrow> 'a \<Rightarrow> bool" (infixr "or" 30) where
-  "a or b \<equiv> \<lambda>s. a s \<or> b s"
-
-abbreviation (input)
-  pred_not :: "('a \<Rightarrow> bool) \<Rightarrow> 'a \<Rightarrow> bool" ("not _" [40] 40) where
-  "not a \<equiv> \<lambda>s. \<not>a s"
-
-abbreviation (input)
-  pred_imp :: "('a \<Rightarrow> bool) \<Rightarrow> ('a \<Rightarrow> bool) \<Rightarrow> 'a \<Rightarrow> bool" (infixr "imp" 25) where
-  "a imp b \<equiv> \<lambda>s. a s \<longrightarrow> b s"
-
-abbreviation (input)
-  pred_iff :: "('a \<Rightarrow> bool) \<Rightarrow> ('a \<Rightarrow> bool) \<Rightarrow> 'a \<Rightarrow> bool" (infixr "iff" 25) where
-  "a iff b \<equiv> \<lambda>s. a s \<longleftrightarrow> b s"
 
 abbreviation (input)
   pred_K :: "'b \<Rightarrow> 'a \<Rightarrow> 'b" ("\<langle>_\<rangle>") where
   "\<langle>f\<rangle> \<equiv> \<lambda>s. f"
 
 abbreviation (input)
-  pred_conjoin :: "('a \<Rightarrow> bool) list \<Rightarrow> 'a \<Rightarrow> bool" where
-  "pred_conjoin xs \<equiv> foldr (and) xs \<langle>True\<rangle>"
+  pred_not :: "('a \<Rightarrow> bool) \<Rightarrow> 'a \<Rightarrow> bool" ("\<^bold>\<not>") where
+  "\<^bold>\<not>a \<equiv> \<lambda>s. \<not>a s"
 
 abbreviation (input)
-  pred_singleton :: "('a \<Rightarrow> 'b) \<Rightarrow> 'a \<Rightarrow> 'b set" where
-  "pred_singleton x \<equiv> \<lambda>s. {x s}"
+  pred_conj :: "('a \<Rightarrow> bool) \<Rightarrow> ('a \<Rightarrow> bool) \<Rightarrow> 'a \<Rightarrow> bool" (infixr "\<^bold>\<and>" 35) where
+  "a \<^bold>\<and> b \<equiv> \<lambda>s. a s \<and> b s"
 
 abbreviation (input)
-  pred_empty :: "('a \<Rightarrow> 'b set) \<Rightarrow> 'a \<Rightarrow> bool" ("empty _" [40] 40) where
-  "empty a \<equiv> \<lambda>s. a s = {}"
+  pred_disj :: "('a \<Rightarrow> bool) \<Rightarrow> ('a \<Rightarrow> bool) \<Rightarrow> 'a \<Rightarrow> bool" (infixr "\<^bold>\<or>" 30) where
+  "a \<^bold>\<or> b \<equiv> \<lambda>s. a s \<or> b s"
 
 abbreviation (input)
-  pred_map_empty :: "('a \<Rightarrow> ('b \<Rightarrow> 'c option)) \<Rightarrow> 'a \<Rightarrow> bool" ("map'_empty _" [40] 40) where
-  "map_empty a \<equiv> \<lambda>s. a s = Map.empty"
+  pred_implies :: "('a \<Rightarrow> bool) \<Rightarrow> ('a \<Rightarrow> bool) \<Rightarrow> 'a \<Rightarrow> bool" (infixr "\<^bold>\<longrightarrow>" 25) where
+  "a \<^bold>\<longrightarrow> b \<equiv> \<lambda>s. a s \<longrightarrow> b s"
 
 abbreviation (input)
-  pred_list_null :: "('a \<Rightarrow> 'b list) \<Rightarrow> 'a \<Rightarrow> bool" ("list'_null _" [40] 40) where
-  "list_null a \<equiv> \<lambda>s. a s = []"
+  pred_eq :: "('a \<Rightarrow> 'b) \<Rightarrow> ('a \<Rightarrow> 'b) \<Rightarrow> 'a \<Rightarrow> bool" (infix "\<^bold>=" 40) where
+  "a \<^bold>= b \<equiv> \<lambda>s. a s = b s"
 
 abbreviation (input)
-  pred_null :: "('a \<Rightarrow> 'b option) \<Rightarrow> 'a \<Rightarrow> bool" ("null _" [40] 40) where
-  "null a \<equiv> \<lambda>s. a s = None"
+  pred_member :: "('a \<Rightarrow> 'b) \<Rightarrow> ('a \<Rightarrow> 'b set) \<Rightarrow> 'a \<Rightarrow> bool" (infix "\<^bold>\<in>" 40) where
+  "a \<^bold>\<in> b \<equiv> \<lambda>s. a s \<in> b s"
 
 abbreviation (input)
-  pred_ex :: "('b \<Rightarrow> 'a \<Rightarrow> bool) \<Rightarrow> 'a \<Rightarrow> bool" (binder "EXS " 10) where
-  "EXS x. P x \<equiv> \<lambda>s. \<exists>x. P x s"
-
-abbreviation (input)
-  pred_all :: "('b \<Rightarrow> 'a \<Rightarrow> bool) \<Rightarrow> 'a \<Rightarrow> bool" (binder "ALLS " 10) where
-  "ALLS x. P x \<equiv> \<lambda>s. \<forall>x. P x s"
+  pred_neq :: "('a \<Rightarrow> 'b) \<Rightarrow> ('a \<Rightarrow> 'b) \<Rightarrow> 'a \<Rightarrow> bool" (infix "\<^bold>\<noteq>" 40) where
+  "a \<^bold>\<noteq> b \<equiv> \<lambda>s. a s \<noteq> b s"
 
 abbreviation (input)
   pred_If :: "('a \<Rightarrow> bool) \<Rightarrow> ('a \<Rightarrow> 'b) \<Rightarrow> ('a \<Rightarrow> 'b) \<Rightarrow> 'a \<Rightarrow> 'b" ("(If (_)/ Then (_)/ Else (_))" [0, 0, 10] 10)
   where "If P Then x Else y \<equiv> \<lambda>s. if P s then x s else y s"
+
+abbreviation (input)
+  pred_less :: "('a \<Rightarrow> 'b::ord) \<Rightarrow> ('a \<Rightarrow> 'b) \<Rightarrow> 'a \<Rightarrow> bool" (infix "\<^bold><" 40) where
+  "a \<^bold>< b \<equiv> \<lambda>s. a s < b s"
+
+abbreviation (input)
+  pred_le :: "('a \<Rightarrow> 'b::ord) \<Rightarrow> ('a \<Rightarrow> 'b) \<Rightarrow> 'a \<Rightarrow> bool" (infix "\<^bold>\<le>" 40) where
+  "a \<^bold>\<le> b \<equiv> \<lambda>s. a s \<le> b s"
+
+abbreviation (input)
+  pred_plus :: "('a \<Rightarrow> 'b::plus) \<Rightarrow> ('a \<Rightarrow> 'b) \<Rightarrow> 'a \<Rightarrow> 'b" (infixl "\<^bold>+" 65) where
+  "a \<^bold>+ b \<equiv> \<lambda>s. a s + b s"
+
+abbreviation (input)
+  pred_minus :: "('a \<Rightarrow> 'b::minus) \<Rightarrow> ('a \<Rightarrow> 'b) \<Rightarrow> 'a \<Rightarrow> 'b" (infixl "\<^bold>-" 65) where
+  "a \<^bold>- b \<equiv> \<lambda>s. a s - b s"
+
+abbreviation (input)
+  fun_fanout :: "('a \<Rightarrow> 'b) \<Rightarrow> ('a \<Rightarrow> 'c) \<Rightarrow> 'a \<Rightarrow> 'b \<times> 'c" (infix "\<^bold>\<bowtie>" 35) where
+  "f \<^bold>\<bowtie> g \<equiv> \<lambda>x. (f x, g x)"
+
+abbreviation (input)
+  pred_all :: "('b \<Rightarrow> 'a \<Rightarrow> bool) \<Rightarrow> 'a \<Rightarrow> bool" (binder "\<^bold>\<forall>" 10) where
+  "\<^bold>\<forall>x. P x \<equiv> \<lambda>s. \<forall>x. P x s"
+
+abbreviation (input)
+  pred_ex :: "('b \<Rightarrow> 'a \<Rightarrow> bool) \<Rightarrow> 'a \<Rightarrow> bool" (binder "\<^bold>\<exists>" 10) where
+  "\<^bold>\<exists>x. P x \<equiv> \<lambda>s. \<exists>x. P x s"
+
+abbreviation (input)
+  pred_app :: "('b \<Rightarrow> 'a \<Rightarrow> 'c) \<Rightarrow> ('a \<Rightarrow> 'b) \<Rightarrow> 'a \<Rightarrow> 'c" (infixl "\<^bold>$" 100) where
+  "f \<^bold>$ g \<equiv> \<lambda>s. f (g s) s"
+
+abbreviation (input)
+  pred_subseteq :: "('a \<Rightarrow> 'b set) \<Rightarrow> ('a \<Rightarrow> 'b set) \<Rightarrow> 'a \<Rightarrow> bool" (infix "\<^bold>\<subseteq>" 50) where
+  "A \<^bold>\<subseteq> B \<equiv> \<lambda>s. A s \<subseteq> B s"
+
+abbreviation (input)
+  pred_union :: "('a \<Rightarrow> 'b set) \<Rightarrow> ('a \<Rightarrow> 'b set) \<Rightarrow> 'a \<Rightarrow> 'b set" (infixl "\<^bold>\<union>" 65) where
+  "a \<^bold>\<union> b \<equiv> \<lambda>s. a s \<union> b s"
+
+text\<open>
+
+More application specific.
+
+\<close>
+
+abbreviation (input)
+  pred_conjoin :: "('a \<Rightarrow> bool) list \<Rightarrow> 'a \<Rightarrow> bool" where
+  "pred_conjoin xs \<equiv> foldr (\<^bold>\<and>) xs \<langle>True\<rangle>"
+
+abbreviation (input)
+  pred_is_none :: "('a \<Rightarrow> 'b option) \<Rightarrow> 'a \<Rightarrow> bool" ("NULL _" [40] 40) where
+  "NULL a \<equiv> \<lambda>s. a s = None"
+
+abbreviation (input)
+  pred_empty :: "('a \<Rightarrow> 'b set) \<Rightarrow> 'a \<Rightarrow> bool" ("EMPTY _" [40] 40) where
+  "EMPTY a \<equiv> \<lambda>s. a s = {}"
+
+abbreviation (input)
+  pred_list_null :: "('a \<Rightarrow> 'b list) \<Rightarrow> 'a \<Rightarrow> bool" ("LIST'_NULL _" [40] 40) where
+  "LIST_NULL a \<equiv> \<lambda>s. a s = []"
+
+abbreviation (input)
+  pred_pair :: "('a \<Rightarrow> 'b) \<Rightarrow> ('a \<Rightarrow> 'c) \<Rightarrow> 'a \<Rightarrow> 'b \<times> 'c" (infixr "\<^bold>\<otimes>" 60) where
+  "a \<^bold>\<otimes> b \<equiv> \<lambda>s. (a s, b s)"
+
+abbreviation (input)
+  pred_singleton :: "('a \<Rightarrow> 'b) \<Rightarrow> 'a \<Rightarrow> 'b set" where
+  "pred_singleton x \<equiv> \<lambda>s. {x s}"
 (*<*)
 
 end
